RealTimeDeque: Separate implementation and auxiliary functions

thys/Real_Time_Deque/Big.thy
@@ -18,24 +18,8 @@ datatype (plugins del: size) 'a state =
 
 text \<open>\<^noindent> Functions:
 
-\<^descr> \<open>step\<close>: Executes one step of the transformation
-\<^descr> \<open>size_new\<close>: Returns the size that the deque end will have after the transformation is finished.
-\<^descr> \<open>size\<close>: Minimum of \<open>size_new\<close> and the number of elements contained in the current state.
-\<^descr> \<open>remaining_steps\<close>: Returns how many steps are left until the transformation is finished.
-\<^descr> \<open>list\<close>: List abstraction of the elements which this end will contain after the transformation is finished
-\<^descr> \<open>list_current\<close>: List abstraction of the elements currently in this deque end.
-\<close>
-
-fun list :: "'a state \<Rightarrow> 'a list" where
-  "list (Common common) = Common.list common"
-| "list (Reverse (Current extra _ _ remained) big aux count) = (
-   let reversed = reverseN count (Stack.list big) aux in
-    extra @ (reverseN remained reversed [])
-  )"
-
-fun list_current :: "'a state \<Rightarrow> 'a list" where
-  "list_current (Common common) = Common.list_current common"
-| "list_current (Reverse current _ _ _) = Current.list current"
+\<^descr> \<open>push\<close>, \<open>pop\<close>: Add and remove elements using the \<open>current\<close> state.
+\<^descr> \<open>step\<close>: Executes one step of the transformation\<close>
 
 instantiation state ::(type) step
 begin
@@ -56,66 +40,5 @@ fun push :: "'a \<Rightarrow> 'a state \<Rightarrow> 'a state" where
 fun pop :: "'a state \<Rightarrow> 'a * 'a state" where
   "pop (Common state) = (let (x, state) = Common.pop state in (x, Common state))"
 | "pop (Reverse current big aux count) = (first current, Reverse (drop_first current) big aux count)"
-
-instantiation state ::(type) is_empty
-begin
-
-fun is_empty_state :: "'a state \<Rightarrow> bool" where
-  "is_empty (Common state) = is_empty state"
-| "is_empty (Reverse current _ _ count) = (
-    case current of Current extra added old remained \<Rightarrow> 
-      is_empty current \<or> remained \<le> count
-)"
-
-instance..
-end
-
-instantiation state ::(type) invar
-begin
-
-fun invar_state :: "'a state \<Rightarrow> bool" where
-  "invar (Common state) \<longleftrightarrow> invar state"
-| "invar (Reverse current big aux count) \<longleftrightarrow> (
-   case current of Current extra added old remained \<Rightarrow>
-      invar current
-    \<and> List.length aux \<ge> remained - count
-    
-    \<and> count \<le> size big
-    \<and> Stack.list old = rev (take (size old) ((rev (Stack.list big)) @ aux))
-    \<and> take remained (Stack.list old) = rev (take remained (reverseN count (Stack.list big) aux))
-)"
-
-instance..
-end
-
-instantiation state ::(type) size
-begin
-
-fun size_state :: "'a state \<Rightarrow> nat" where
-  "size (Common state) = size state"
-| "size (Reverse current _ _ _) = min (size current) (size_new current)"
-
-instance..
-end
-
-instantiation state ::(type) size_new
-begin
-
-fun size_new_state :: "'a state \<Rightarrow> nat" where
-  "size_new (Common state) = size_new state"
-| "size_new (Reverse current _ _ _) = size_new current"
-
-instance..
-end
-
-instantiation state ::(type) remaining_steps
-begin
-
-fun remaining_steps_state :: "'a state \<Rightarrow> nat" where
-  "remaining_steps (Common state) = remaining_steps state"
-| "remaining_steps (Reverse (Current _ _ _ remaining) _ _ count) = count + remaining + 1"
-
-instance..
-end
 
 end
