thys/Real_Time_Deque/Common.thy
@@ -21,30 +21,7 @@ text\<open>
 \<^noindent> Functions:
 
 \<^descr> \<open>push\<close>, \<open>pop\<close>: Add and remove elements using the \<open>current\<close> state.
-\<^descr> \<open>list\<close>: List abstraction of the elements which this end will contain after the transformation is finished
-\<^descr> \<open>list_current\<close>: List abstraction of the elements currently in this deque end.
-\<^descr> \<open>step\<close>: Executes one step of the transformation, while keeping the invariant.
-\<^descr> \<open>remaining_steps\<close>: Returns how many steps are left until the transformation is finished.
-\<^descr> \<open>size_new\<close>: Returns the size, that the deque end will have after the transformation is finished.
-\<^descr> \<open>size\<close>: Minimum of \<open>size_new\<close> and the number of elements contained in the \<open>current\<close> state.
-\<close>
-(*
-fun reverseN :: "nat \<Rightarrow> 'a list \<Rightarrow> 'a list \<Rightarrow> 'a list" where
-  "reverseN 0 xs acc = acc"
-| "reverseN n [] acc = acc"
-| "reverseN (Suc n) (x#xs) acc = reverseN n xs (x#acc)"
-*)
-definition reverseN where
-[simp]:  "reverseN n xs acc \<equiv> rev (take n xs) @ acc"
-
-fun list :: "'a state \<Rightarrow> 'a list" where
-  "list (Idle _ idle) = Idle.list idle"
-| "list (Copy (Current extra _ _ remained) old new moved) 
-   = extra @ reverseN (remained - moved) old new"
-
-fun list_current :: "'a state \<Rightarrow> 'a list" where
-  "list_current (Idle current _) = Current.list current"
-| "list_current (Copy current _ _ _) = Current.list current"
+\<^descr> \<open>step\<close>: Executes one step of the transformation, while keeping the invariant.\<close>
 
 (* TODO: Maybe inline function? *)
 fun normalize :: "'a state \<Rightarrow> 'a state" where
@@ -83,68 +60,5 @@ fun pop :: "'a state \<Rightarrow> 'a * 'a state" where
   "pop (Idle current idle) = (let (x, idle) = Idle.pop idle in (x, Idle (drop_first current) idle))"
 | "pop (Copy current aux new moved) = 
       (first current, normalize (Copy (drop_first current) aux new moved))"
-
-instantiation state ::(type) is_empty
-begin
-
-fun is_empty_state :: "'a state \<Rightarrow> bool" where
-  "is_empty (Idle current idle)  \<longleftrightarrow> is_empty current \<or> is_empty idle"
-| "is_empty (Copy current _ _ _) \<longleftrightarrow> is_empty current"
-
-instance..
-end
-
-instantiation state::(type) invar
-begin
-
-fun invar_state :: "'a state \<Rightarrow> bool" where
-  "invar (Idle current idle) \<longleftrightarrow>
-      invar idle 
-    \<and> invar current 
-    \<and> size_new current = size idle
-    \<and> take (size idle) (Current.list current) = 
-      take (size current) (Idle.list idle)"
-| "invar (Copy current aux new moved) \<longleftrightarrow> (
-    case current of Current _ _ old remained \<Rightarrow>
-      moved < remained
-    \<and> moved = length new
-    \<and> remained \<le> length aux + moved
-    \<and> invar current
-    \<and> take remained (Stack.list old) = take (size old) (reverseN (remained - moved) aux new)
- )"
-
-instance..
-end
-
-instantiation state::(type) size
-begin
-
-(* Use size for emptiness? *)
-fun size_state :: "'a state \<Rightarrow> nat" where
-  "size (Idle current idle) = min (size current) (size idle)"
-| "size (Copy current _ _ _) = min (size current) (size_new current)"
-
-instance..
-end
-
-instantiation state::(type) size_new
-begin
-
-fun size_new_state :: "'a state \<Rightarrow> nat" where
-  "size_new (Idle current _) = size_new current"
-| "size_new (Copy current _ _ _) = size_new current"
-
-instance..
-end
-
-instantiation state::(type) remaining_steps
-begin
-
-fun remaining_steps_state :: "'a state \<Rightarrow> nat" where
-  "remaining_steps (Idle _ _) = 0"
-| "remaining_steps (Copy (Current _ _ _ remained) aux new moved) = remained - moved"
-
-instance..
-end
 
 end
