thys/Real_Time_Deque/Current.thy
@@ -14,13 +14,6 @@ text \<open>
 
 datatype (plugins del: size) 'a current = Current "'a list" nat "'a stack" nat
 
-text \<open>Specification functions:
-\<^descr> \<open>list\<close>: list abstraction for the originally contained elements of a deque end during transformation.
-\<^descr> \<open>invar\<close>: Is the stored number of newly added elements correct?
-\<^descr> \<open>size\<close>: The number of the originally contained elements.
-\<^descr> \<open>size_new\<close>: Number of elements which will be contained after the transformation is finished.
-\<close>
-
 fun push :: "'a \<Rightarrow> 'a current \<Rightarrow> 'a current" where
   "push x (Current extra added old remained) = Current (x#extra) (added + 1) old remained"
 
@@ -33,45 +26,5 @@ fun first :: "'a current \<Rightarrow> 'a" where
 
 abbreviation drop_first :: "'a current \<Rightarrow> 'a current" where
   "drop_first current \<equiv> snd (pop current)"
-
-fun list :: "'a current \<Rightarrow> 'a list" where
-  "list (Current extra _ old _) = extra @ (Stack.list old)"
-
-instantiation current::(type) is_empty
-begin
-
-(* TODO: Actually it should be "added + remained = 0" Maybe directly base it on size? *) 
-fun is_empty_current :: "'a current \<Rightarrow> bool" where
-  "is_empty (Current extra _ old remained) \<longleftrightarrow> is_empty old \<and> extra = [] \<or> remained = 0"
-
-instance..
-end
-
-instantiation current::(type) invar
-begin
-
-fun invar_current :: "'a current \<Rightarrow> bool" where
-  "invar (Current extra added _ _) \<longleftrightarrow> length extra = added"
-
-instance..
-end
-
-instantiation current::(type) size
-begin
-
-fun size_current :: "'a current \<Rightarrow> nat" where
-  "size (Current _ added old _) = added + size old"
-
-instance..
-end
-
-instantiation current::(type) size_new
-begin
-
-fun size_new_current :: "'a current \<Rightarrow> nat" where
-  "size_new (Current _ added _ remained) = added + remained"
-
-instance..
-end
 
 end
