thys/Real_Time_Deque/Idle.thy
@@ -9,40 +9,10 @@ It contains a \<open>stack\<close> and its size as a natural number.\<close>
 
 datatype (plugins del: size) 'a idle = Idle "'a stack" nat
 
-fun list :: "'a idle \<Rightarrow> 'a list" where
-  "list (Idle stack _) = Stack.list stack"
-
 fun push :: "'a \<Rightarrow> 'a idle \<Rightarrow> 'a idle" where
   "push x (Idle stack stackSize) = Idle (Stack.push x stack) (Suc stackSize)"
 
 fun pop :: "'a idle \<Rightarrow> ('a * 'a idle)" where
   "pop (Idle stack stackSize) = (Stack.first stack, Idle (Stack.pop stack) (stackSize - 1))"
-
-instantiation idle :: (type) size
-begin
-
-fun size_idle :: "'a idle \<Rightarrow> nat" where
-  "size (Idle stack _) = size stack"
-
-instance..
-end
-
-instantiation idle :: (type) is_empty
-begin
-
-fun is_empty_idle :: "'a idle \<Rightarrow> bool" where
-  "is_empty (Idle stack _) \<longleftrightarrow> is_empty stack"
-
-instance..
-end
-
-instantiation idle ::(type) invar
-begin
-
-fun invar_idle :: "'a idle \<Rightarrow> bool" where
-  "invar (Idle stack stackSize) \<longleftrightarrow> size stack = stackSize"
-
-instance..
-end
   
 end
