thys/Real_Time_Deque/RealTimeDeque.thy
@@ -188,41 +188,5 @@ fun enqR :: "'a \<Rightarrow> 'a deque \<Rightarrow> 'a deque" where
     let deque = enqL x (swap deque) 
     in swap deque
   )"    
- 
-fun listL :: "'a deque \<Rightarrow> 'a list" where
-  "listL Empty = []"
-| "listL (One x) = [x]"
-| "listL (Two x y) = [x, y]"
-| "listL (Three x y z) = [x, y, z]"
-| "listL (Idle left right) = Idle.list left @ (rev (Idle.list right))"
-| "listL (Transforming states) = States.listL states"
-
-abbreviation listR :: "'a deque \<Rightarrow> 'a list" where
-  "listR deque \<equiv> rev (listL deque)"
-
-instantiation deque::(type) invar
-begin
-
-fun invar_deque :: "'a deque \<Rightarrow> bool" where
-  "invar Empty = True"
-| "invar (One _) = True"
-| "invar (Two _ _) = True"
-| "invar (Three _ _ _) = True"
-| "invar (Idle left right) \<longleftrightarrow>
-   invar left  \<and>
-   invar right \<and>
-   \<not> is_empty left  \<and> 
-   \<not> is_empty right \<and>
-   3 * size right \<ge> size left \<and>
-   3 * size left \<ge> size right
-  "
-| "invar (Transforming states) \<longleftrightarrow> 
-   invar states \<and>
-   size_ok states \<and>
-   0 < remaining_steps states
-  "
-
-instance..
-end
 
 end
