thys/Real_Time_Deque/Stack.thy
@@ -10,10 +10,6 @@ The function \<open>list\<close> appends the two lists and is needed for the lis
 
 datatype (plugins del: size) 'a stack = Stack "'a list" "'a list"
 
-(* TODO: Move into emptyable? *)
-definition empty where
-  "empty \<equiv> Stack [] []"
-
 fun push :: "'a \<Rightarrow> 'a stack \<Rightarrow> 'a stack" where
   "push x (Stack left right) = Stack (x#left) right"
 
@@ -26,24 +22,12 @@ fun first :: "'a stack \<Rightarrow> 'a" where
   "first (Stack (x#left) right)     = x"
 | "first (Stack []       (x#right)) = x"
 
-fun list :: "'a stack \<Rightarrow> 'a list" where
-  "list (Stack left right) = left @ right"
-
 instantiation stack ::(type) is_empty
 begin
 
 fun is_empty_stack where
   "is_empty_stack (Stack [] []) = True" 
 | "is_empty_stack _             = False"
-
-instance..
-end
-
-instantiation stack ::(type) size
-begin
-
-fun size_stack :: "'a stack \<Rightarrow> nat" where
-  "size (Stack left right) = length left + length right"
 
 instance..
 end
