thys/Real_Time_Deque/Big_Aux.thy
@@ -1,0 +1,73 @@
+theory Big_Aux
+imports Big Common_Aux
+begin    
+
+text \<open>\<^noindent> Functions:
+
+\<^descr> \<open>size_new\<close>: Returns the size that the deque end will have after the transformation is finished.
+\<^descr> \<open>size\<close>: Minimum of \<open>size_new\<close> and the number of elements contained in the current state.
+\<^descr> \<open>remaining_steps\<close>: Returns how many steps are left until the transformation is finished.
+\<^descr> \<open>list\<close>: List abstraction of the elements which this end will contain after the transformation is finished
+\<^descr> \<open>list_current\<close>: List abstraction of the elements currently in this deque end.\<close>
+
+fun list :: "'a state \<Rightarrow> 'a list" where
+  "list (Common common) = Common_Aux.list common"
+| "list (Reverse (Current extra _ _ remained) big aux count) = (
+   let reversed = reverseN count (Stack_Aux.list big) aux in
+    extra @ (reverseN remained reversed [])
+  )"
+
+fun list_current :: "'a state \<Rightarrow> 'a list" where
+  "list_current (Common common) = Common_Aux.list_current common"
+| "list_current (Reverse current _ _ _) = Current_Aux.list current"
+
+instantiation state ::(type) invar
+begin
+
+fun invar_state :: "'a state \<Rightarrow> bool" where
+  "invar (Common state) \<longleftrightarrow> invar state"
+| "invar (Reverse current big aux count) \<longleftrightarrow> (
+   case current of Current extra added old remained \<Rightarrow>
+      invar current
+    \<and> List.length aux \<ge> remained - count
+    
+    \<and> count \<le> size big
+    \<and> Stack_Aux.list old = rev (take (size old) ((rev (Stack_Aux.list big)) @ aux))
+    \<and> take remained (Stack_Aux.list old) = 
+      rev (take remained (reverseN count (Stack_Aux.list big) aux))
+)"
+
+instance..
+end
+
+instantiation state ::(type) size
+begin
+
+fun size_state :: "'a state \<Rightarrow> nat" where
+  "size (Common state) = size state"
+| "size (Reverse current _ _ _) = min (size current) (size_new current)"
+
+instance..
+end
+
+instantiation state ::(type) size_new
+begin
+
+fun size_new_state :: "'a state \<Rightarrow> nat" where
+  "size_new (Common state) = size_new state"
+| "size_new (Reverse current _ _ _) = size_new current"
+
+instance..
+end
+
+instantiation state ::(type) remaining_steps
+begin
+
+fun remaining_steps_state :: "'a state \<Rightarrow> nat" where
+  "remaining_steps (Common state) = remaining_steps state"
+| "remaining_steps (Reverse (Current _ _ _ remaining) _ _ count) = count + remaining + 1"
+
+instance..
+end
+
+end
