thys/Real_Time_Deque/Big_Proof.thy
@@ -1,7 +1,7 @@
 section "Big Proofs"
 
 theory Big_Proof
-imports Big Common_Proof
+imports Big_Aux Common_Proof
 begin
 
 lemma step_list [simp]: "invar big \<Longrightarrow> list (step big) = list big"
@@ -40,28 +40,28 @@ lemma list_Reverse: "\<lbrakk>
       list (Reverse current big aux count)" 
 proof(induction current rule: Current.pop.induct)
   case (1 added old remained)
-  then have [simp]: "remained - Suc 0 < length (reverseN count (Stack.list big) aux)"
+  then have [simp]: "remained - Suc 0 < length (reverseN count (Stack_Aux.list big) aux)"
     by(auto simp: le_diff_conv)
 
   (* TODO: *)
   then have "
    \<lbrakk>0 < size old; 0 < remained; added = 0; remained - count \<le> length aux; count \<le> size big;
-     Stack.list old =
-     rev (take (size old - size big) aux) @ rev (take (size old) (rev (Stack.list big)));
+     Stack_Aux.list old =
+     rev (take (size old - size big) aux) @ rev (take (size old) (rev (Stack_Aux.list big)));
      take remained (rev (take (size old - size big) aux)) @
      take (remained - min (length aux) (size old - size big))
-      (rev (take (size old) (rev (Stack.list big)))) =
-     rev (take (remained - count) aux) @ rev (take remained (rev (take count (Stack.list big))))\<rbrakk>
-    \<Longrightarrow> hd (rev (take (size old - size big) aux) @ rev (take (size old) (rev (Stack.list big)))) =
-        (rev (take count (Stack.list big)) @ aux) ! (remained - Suc 0)"
+      (rev (take (size old) (rev (Stack_Aux.list big)))) =
+     rev (take (remained - count) aux) @ rev (take remained (rev (take count (Stack_Aux.list big))))\<rbrakk>
+    \<Longrightarrow> hd (rev (take (size old - size big) aux) @ rev (take (size old) (rev (Stack_Aux.list big)))) =
+        (rev (take count (Stack_Aux.list big)) @ aux) ! (remained - Suc 0)"
     by (smt (verit) Suc_pred hd_drop_conv_nth hd_rev hd_take last_snoc length_rev length_take min.absorb2 rev_append reverseN_def size_list_length take_append take_hd_drop)
 
-  with 1 have [simp]: "Stack.first old = reverseN count (Stack.list big) aux ! (remained - Suc 0)"
+  with 1 have [simp]: "Stack.first old = reverseN count (Stack_Aux.list big) aux ! (remained - Suc 0)"
     by(auto simp: take_hd_drop first_hd)
  
   from 1 show ?case
     using reverseN_nth[of 
-          "remained - Suc 0" "reverseN count (Stack.list big) aux" "Stack.first old" "[]"
+          "remained - Suc 0" "reverseN count (Stack_Aux.list big) aux" "Stack.first old" "[]"
         ]
     by auto
 next
@@ -92,8 +92,7 @@ next
     by (metis Big.pop.simps(2) list_Reverse prod.inject)
 qed
 
-lemma pop_list_tl: "\<lbrakk>0 < size big; invar big; Big.pop big = (x, big')\<rbrakk>
-   \<Longrightarrow> Big.list big' = tl (Big.list big)"
+lemma pop_list_tl: "\<lbrakk>0 < size big; invar big; pop big = (x, big')\<rbrakk> \<Longrightarrow> list big' = tl (list big)"
   using pop_list cons_tl[of x "list big'" "list big"] 
   by force
 
@@ -112,11 +111,11 @@ next
 
   (* TODO: *)
   with 2 have "\<lbrakk>current = Current extra (length extra) old remained; remained \<le> length aux;
-     Stack.list old =
-     rev (take (size old - size big) aux) @ rev (take (size old) (rev (Stack.list big)));
+     Stack_Aux.list old =
+     rev (take (size old - size big) aux) @ rev (take (size old) (rev (Stack_Aux.list big)));
      take remained (rev (take (size old - size big) aux)) @
      take (remained - min (length aux) (size old - size big))
-      (rev (take (size old) (rev (Stack.list big)))) =
+      (rev (take (size old) (rev (Stack_Aux.list big)))) =
      rev (take remained aux)\<rbrakk>
     \<Longrightarrow> remained \<le> size old"
     by(metis length_rev length_take min.absorb_iff2 size_list_length take_append)
@@ -131,21 +130,21 @@ next
   then have "0 < size big"
     by(auto split: current.splits)
 
-  then have big_not_empty:  "Stack.list big \<noteq> []"
+  then have big_not_empty:  "Stack_Aux.list big \<noteq> []"
     by(auto simp: Stack_Proof.size_not_empty  Stack_Proof.list_not_empty)
 
   with 3 have a: "
-      rev (Stack.list big) @ aux =
-      rev (Stack.list (Stack.pop big)) @ Stack.first big # aux"
+      rev (Stack_Aux.list big) @ aux =
+      rev (Stack_Aux.list (Stack.pop big)) @ Stack.first big # aux"
     by(auto simp: rev_tl_hd first_hd split: current.splits)
 
   from 3 have "0 < size big" 
     by(auto split: current.splits)
   
   from 3 big_not_empty have "
-      reverseN (Suc count) (Stack.list big) aux = 
-      reverseN count (Stack.list (Stack.pop big)) (Stack.first big # aux)"
-    using reverseN_tl_hd[of "Suc count" "Stack.list big" aux]
+      reverseN (Suc count) (Stack_Aux.list big) aux = 
+      reverseN count (Stack_Aux.list (Stack.pop big)) (Stack.first big # aux)"
+    using reverseN_tl_hd[of "Suc count" "Stack_Aux.list big" aux]
     by(auto simp: Stack_Proof.list_not_empty split: current.splits)
  
   with 3 a show ?case
@@ -175,35 +174,35 @@ next
 
     have a: " \<lbrakk>remained \<le> count + length aux; 0 < remained; added = 0; x = Stack.first old;
          big' = Reverse (Current [] 0 (Stack.pop old) (remained - Suc 0)) big aux count;
-         count \<le> size big; Stack.list old = rev aux @ Stack.list big;
-         take remained (rev aux) @ take (remained - length aux) (Stack.list big) =
+         count \<le> size big; Stack_Aux.list old = rev aux @ Stack_Aux.list big;
+         take remained (rev aux) @ take (remained - length aux) (Stack_Aux.list big) =
          drop (count + length aux - remained) (rev aux) @
-         drop (count - remained) (take count (Stack.list big));
+         drop (count - remained) (take count (Stack_Aux.list big));
          \<not> size old \<le> length aux + size big\<rbrakk>
-        \<Longrightarrow> tl (rev aux @ Stack.list big) = rev aux @ Stack.list big"
+        \<Longrightarrow> tl (rev aux @ Stack_Aux.list big) = rev aux @ Stack_Aux.list big"
       by (metis le_refl length_append length_rev size_list_length)
 
-    have b: "\<lbrakk>remained \<le> length (reverseN count (Stack.list big) aux); 0 < size old; 
+    have b: "\<lbrakk>remained \<le> length (reverseN count (Stack_Aux.list big) aux); 0 < size old; 
           0 < remained; added = 0;
          x = Stack.first old;
          big' = Reverse (Current [] 0 (Stack.pop old) (remained - Suc 0)) big aux count;
          remained - count \<le> length aux; count \<le> size big;
-         Stack.list old =
+         Stack_Aux.list old =
          drop (length aux - (size old - size big)) (rev aux) @
-         drop (size big - size old) (Stack.list big);
+         drop (size big - size old) (Stack_Aux.list big);
          take remained (drop (length aux - (size old - size big)) (rev aux)) @
          take (remained + (length aux - (size old - size big)) - length aux)
-          (drop (size big - size old) (Stack.list big)) =
-         drop (length (reverseN count (Stack.list big) aux) - remained)
-          (rev (reverseN count (Stack.list big) aux))\<rbrakk>
+          (drop (size big - size old) (Stack_Aux.list big)) =
+         drop (length (reverseN count (Stack_Aux.list big) aux) - remained)
+          (rev (reverseN count (Stack_Aux.list big) aux))\<rbrakk>
         \<Longrightarrow> tl (drop (length aux - (size old - size big)) (rev aux) @
-                drop (size big - size old) (Stack.list big)) =
+                drop (size big - size old) (Stack_Aux.list big)) =
             drop (length aux - (size old - Suc (size big))) (rev aux) @
-            drop (Suc (size big) - size old) (Stack.list big)"
+            drop (Suc (size big) - size old) (Stack_Aux.list big)"
       apply(cases "size old - size big \<le> length aux"; cases "size old \<le> size big")
       by(auto simp: tl_drop_2 Suc_diff_le le_diff_conv le_refl a)
 
-    from 1 have "remained \<le> length (reverseN count (Stack.list big) aux)"
+    from 1 have "remained \<le> length (reverseN count (Stack_Aux.list big) aux)"
       by(auto)
 
     with 1 show ?case 
@@ -219,7 +218,7 @@ lemma push_list_current [simp]: "list_current (push x big) = x # list_current bi
   by(induction x big rule: push.induct) auto
 
 lemma pop_list_current [simp]: "\<lbrakk>invar big; 0 < size big; Big.pop big = (x, big')\<rbrakk>
-   \<Longrightarrow> x # Big.list_current big' = Big.list_current big"
+   \<Longrightarrow> x # list_current big' = list_current big"
 proof(induction big arbitrary: x rule: pop.induct)
   case (1 state)
   then show ?case 
@@ -231,7 +230,7 @@ next
     case (1 added old remained)
   
     then have 
-        "rev (take (size old - size big) aux) @ rev (take (size old) (rev (Stack.list big))) \<noteq> []" 
+        "rev (take (size old - size big) aux) @ rev (take (size old) (rev (Stack_Aux.list big))) \<noteq> []" 
       using 
         order_less_le_trans[of 0 "size old" "size big"] 
         order_less_le_trans[of 0 count "size big"]
@@ -261,17 +260,6 @@ qed
 
 lemma step_size: "invar (big :: 'a state) \<Longrightarrow> size big = size (step big)"
   by(induction big rule: step_state.induct)(auto split: current.splits)
-
-lemma size_empty: "\<lbrakk>invar (big :: 'a state); size big = 0\<rbrakk> \<Longrightarrow> is_empty big"
-proof(induction big)
-  case Reverse
-  then show ?case 
-    by(auto simp: min_def Stack_Proof.list_empty split: if_splits current.splits)
-next
-  case Common
-  then show ?case 
-    by(auto simp: size_empty)
-qed
 
 lemma remaining_steps_step [simp]: "\<lbrakk>invar (big :: 'a state); remaining_steps big > 0\<rbrakk>
    \<Longrightarrow> Suc (remaining_steps (step big)) = remaining_steps big"
