thys/Real_Time_Deque/Common_Aux.thy
@@ -1,0 +1,79 @@
+theory Common_Aux
+imports Common Current_Aux Idle_Aux
+begin
+
+text\<open>
+\<^noindent> Functions:
+
+\<^descr> \<open>list\<close>: List abstraction of the elements which this end will contain after the transformation is finished
+\<^descr> \<open>list_current\<close>: List abstraction of the elements currently in this deque end.
+\<^descr> \<open>remaining_steps\<close>: Returns how many steps are left until the transformation is finished.
+\<^descr> \<open>size_new\<close>: Returns the size, that the deque end will have after the transformation is finished.
+\<^descr> \<open>size\<close>: Minimum of \<open>size_new\<close> and the number of elements contained in the \<open>current\<close> state.\<close>
+
+definition reverseN where
+[simp]:  "reverseN n xs acc \<equiv> rev (take n xs) @ acc"
+
+fun list :: "'a state \<Rightarrow> 'a list" where
+  "list (Idle _ idle) = Idle_Aux.list idle"
+| "list (Copy (Current extra _ _ remained) old new moved) 
+   = extra @ reverseN (remained - moved) old new"
+
+fun list_current :: "'a state \<Rightarrow> 'a list" where
+  "list_current (Idle current _) = Current_Aux.list current"
+| "list_current (Copy current _ _ _) = Current_Aux.list current"
+
+instantiation state::(type) invar
+begin
+
+fun invar_state :: "'a state \<Rightarrow> bool" where
+  "invar (Idle current idle) \<longleftrightarrow>
+      invar idle 
+    \<and> invar current 
+    \<and> size_new current = size idle
+    \<and> take (size idle) (Current_Aux.list current) = 
+      take (size current) (Idle_Aux.list idle)"
+| "invar (Copy current aux new moved) \<longleftrightarrow> (
+    case current of Current _ _ old remained \<Rightarrow>
+      moved < remained
+    \<and> moved = length new
+    \<and> remained \<le> length aux + moved
+    \<and> invar current
+    \<and> take remained (Stack_Aux.list old) = take (size old) (reverseN (remained - moved) aux new)
+ )"
+
+instance..
+end
+
+instantiation state::(type) size
+begin
+
+fun size_state :: "'a state \<Rightarrow> nat" where
+  "size (Idle current idle) = min (size current) (size idle)"
+| "size (Copy current _ _ _) = min (size current) (size_new current)"
+
+instance..
+end
+
+instantiation state::(type) size_new
+begin
+
+fun size_new_state :: "'a state \<Rightarrow> nat" where
+  "size_new (Idle current _) = size_new current"
+| "size_new (Copy current _ _ _) = size_new current"
+
+instance..
+end
+
+instantiation state::(type) remaining_steps
+begin
+
+fun remaining_steps_state :: "'a state \<Rightarrow> nat" where
+  "remaining_steps (Idle _ _) = 0"
+| "remaining_steps (Copy (Current _ _ _ remained) aux new moved) = remained - moved"
+
+instance..
+end
+
+
+end
