thys/Real_Time_Deque/Current_Aux.thy
@@ -1,0 +1,41 @@
+theory Current_Aux
+imports Current Stack_Aux
+begin
+
+text \<open>Specification functions:
+\<^descr> \<open>list\<close>: list abstraction for the originally contained elements of a deque end during transformation.
+\<^descr> \<open>invar\<close>: Is the stored number of newly added elements correct?
+\<^descr> \<open>size\<close>: The number of the originally contained elements.
+\<^descr> \<open>size_new\<close>: Number of elements which will be contained after the transformation is finished.\<close>
+
+fun list :: "'a current \<Rightarrow> 'a list" where
+  "list (Current extra _ old _) = extra @ (Stack_Aux.list old)"
+
+instantiation current::(type) invar
+begin
+
+fun invar_current :: "'a current \<Rightarrow> bool" where
+  "invar (Current extra added _ _) \<longleftrightarrow> length extra = added"
+
+instance..
+end
+
+instantiation current::(type) size
+begin
+
+fun size_current :: "'a current \<Rightarrow> nat" where
+  "size (Current _ added old _) = added + size old"
+
+instance..
+end
+
+instantiation current::(type) size_new
+begin
+
+fun size_new_current :: "'a current \<Rightarrow> nat" where
+  "size_new (Current _ added _ remained) = added + remained"
+
+instance..
+end
+
+end
