thys/Real_Time_Deque/Idle_Aux.thy
@@ -1,0 +1,35 @@
+theory Idle_Aux
+imports Idle Stack_Aux
+begin
+
+fun list :: "'a idle \<Rightarrow> 'a list" where
+  "list (Idle stack _) = Stack_Aux.list stack"
+
+instantiation idle :: (type) size
+begin
+
+fun size_idle :: "'a idle \<Rightarrow> nat" where
+  "size (Idle stack _) = size stack"
+
+instance..
+end
+
+instantiation idle :: (type) is_empty
+begin
+
+fun is_empty_idle :: "'a idle \<Rightarrow> bool" where
+  "is_empty (Idle stack _) \<longleftrightarrow> is_empty stack"
+
+instance..
+end
+
+instantiation idle ::(type) invar
+begin
+
+fun invar_idle :: "'a idle \<Rightarrow> bool" where
+  "invar (Idle stack stackSize) \<longleftrightarrow> size stack = stackSize"
+
+instance..
+end
+
+end
