thys/Real_Time_Deque/RealTimeDeque_Aux.thy
@@ -1,0 +1,46 @@
+theory RealTimeDeque_Aux
+  imports RealTimeDeque States_Aux
+begin
+
+text\<open>
+ \<^descr> \<open>listL\<close>, \<open>listR\<close>: Get all elements of the deque in a list starting at the left or right end. 
+   They are needed as list abstractions for the correctness proofs.
+\<close>
+
+fun listL :: "'a deque \<Rightarrow> 'a list" where
+  "listL Empty = []"
+| "listL (One x) = [x]"
+| "listL (Two x y) = [x, y]"
+| "listL (Three x y z) = [x, y, z]"
+| "listL (Idle left right) = Idle_Aux.list left @ (rev (Idle_Aux.list right))"
+| "listL (Transforming states) = States_Aux.listL states"
+
+abbreviation listR :: "'a deque \<Rightarrow> 'a list" where
+  "listR deque \<equiv> rev (listL deque)"
+
+instantiation deque::(type) invar
+begin
+
+fun invar_deque :: "'a deque \<Rightarrow> bool" where
+  "invar Empty = True"
+| "invar (One _) = True"
+| "invar (Two _ _) = True"
+| "invar (Three _ _ _) = True"
+| "invar (Idle left right) \<longleftrightarrow>
+   invar left  \<and>
+   invar right \<and>
+   \<not> is_empty left  \<and> 
+   \<not> is_empty right \<and>
+   3 * size right \<ge> size left \<and>
+   3 * size left \<ge> size right
+  "
+| "invar (Transforming states) \<longleftrightarrow> 
+   invar states \<and>
+   size_ok states \<and>
+   0 < remaining_steps states
+  "
+
+instance..
+end
+
+end
