thys/Real_Time_Deque/Stack_Aux.thy
@@ -1,0 +1,17 @@
+theory Stack_Aux
+imports Stack
+begin
+
+fun list :: "'a stack \<Rightarrow> 'a list" where
+  "list (Stack left right) = left @ right"
+
+instantiation stack ::(type) size
+begin
+
+fun size_stack :: "'a stack \<Rightarrow> nat" where
+  "size (Stack left right) = length left + length right"
+
+instance..
+end
+
+end
