thys/Real_Time_Deque/States_Aux.thy
@@ -1,0 +1,88 @@
+theory States_Aux
+imports States Big_Aux Small_Aux
+begin
+
+instantiation states::(type) remaining_steps
+begin
+
+fun remaining_steps_states :: "'a states \<Rightarrow> nat" where
+  "remaining_steps (States _ big small) = max 
+    (remaining_steps big) 
+    (case small of 
+       Small.Common common \<Rightarrow> remaining_steps common
+     | Reverse2 (Current _ _ _ remaining) _ big _ count \<Rightarrow> (remaining - (count + size big)) + size big + 1
+     | Reverse1 (Current _ _ _ remaining) _ _ \<Rightarrow>
+         case big of
+           Reverse currentB big auxB count \<Rightarrow> size big + (remaining + count - size big) + 2
+    )"
+
+instance..
+end
+
+fun lists :: "'a states \<Rightarrow> 'a list * 'a list" where
+  "lists (States _ (Reverse currentB big auxB count) (Reverse1 currentS small auxS)) = (
+    Big_Aux.list (Reverse currentB big auxB count),
+    Small_Aux.list (Reverse2 currentS (reverseN count (Stack_Aux.list small) auxS) ((Stack.pop ^^ count) big) [] 0)
+  )"
+| "lists (States _ big small) = (Big_Aux.list big, Small_Aux.list small)"
+
+fun list_small_first :: "'a states \<Rightarrow> 'a list" where
+  "list_small_first states = (let (big, small) = lists states in small @ (rev big))"
+
+fun list_big_first :: "'a states \<Rightarrow> 'a list" where
+  "list_big_first states = (let (big, small) = lists states in big @ (rev small))"
+
+fun lists_current :: "'a states \<Rightarrow> 'a list * 'a list" where
+  "lists_current (States _ big small) = (Big_Aux.list_current big, Small_Aux.list_current small)"
+
+fun list_current_small_first :: "'a states \<Rightarrow> 'a list" where
+  "list_current_small_first states = (let (big, small) = lists_current states in small @ (rev big))"
+
+fun list_current_big_first :: "'a states \<Rightarrow> 'a list" where
+  "list_current_big_first states = (let (big, small) = lists_current states in big @ (rev small))"
+
+fun listL :: "'a states \<Rightarrow> 'a list" where
+  "listL (States Left big small)  = list_small_first (States Left big small)"
+| "listL (States Right big small) = list_big_first (States Right big small)"
+
+instantiation states::(type) invar
+begin
+
+fun invar_states :: "'a states \<Rightarrow> bool" where
+  "invar (States dir big small)  \<longleftrightarrow> (
+     invar big 
+   \<and> invar small
+   \<and> list_small_first (States dir big small) = list_current_small_first (States dir big small)
+   \<and> (case (big, small) of 
+        (Reverse _ big _ count, Reverse1 (Current _ _ old remained) small _) \<Rightarrow> 
+          size big - count = remained - size old \<and> count \<ge> size small
+      | (_, Reverse1 _ _ _) \<Rightarrow> False
+      | (Reverse _ _ _ _, _) \<Rightarrow> False
+      | _ \<Rightarrow> True
+      ))"
+
+instance..
+end
+
+fun size_ok' :: "'a states \<Rightarrow> nat \<Rightarrow> bool" where
+  "size_ok' (States _ big small) steps \<longleftrightarrow> 
+      size_new small + steps + 2 \<le> 3 * size_new big
+    \<and> size_new big + steps + 2 \<le> 3 * size_new small
+    \<and> steps + 1 \<le> 4 * size small
+    \<and> steps + 1 \<le> 4 * size big
+  "
+
+abbreviation size_ok :: "'a states \<Rightarrow> bool" where
+  "size_ok states \<equiv> size_ok' states (remaining_steps states)"
+
+abbreviation size_small where "size_small states \<equiv> case states of States _ _ small \<Rightarrow> size small"
+
+abbreviation size_new_small where 
+  "size_new_small states \<equiv> case states of States _ _ small \<Rightarrow> size_new small"
+
+abbreviation size_big where "size_big states \<equiv> case states of States _ big _ \<Rightarrow> size big"
+
+abbreviation size_new_big where 
+  "size_new_big states \<equiv> case states of States _ big _ \<Rightarrow> size_new big"
+
+end
